Make MlirType a String
While this is not the end-goal with MlirType, it allows us to use it
in the parser and the printer, and allows us to catch some bugs in the
codebase that relied on the fact that all types are equal.

Veir/Rewriter/Basic.lean
@@ -357,36 +357,41 @@ theorem Rewriter.initOpRegions_inBounds_mono (ptr : GenericPtr) :
     ptr.InBounds ctx → ptr.InBounds (initOpRegions ctx opPtr regions n opPtrInBounds hregions hctx hn) := by
   induction n generalizing ctx <;> simp only [initOpRegions] <;> grind
 
-@[irreducible]
-def Rewriter.initOpResults (ctx: IRContext) (opPtr: OperationPtr) (numResults: Nat) (index: Nat := 0) (hop : opPtr.InBounds ctx)
+def Rewriter.initOpResults (ctx: IRContext) (opPtr: OperationPtr) (resultTypes: Array MlirType) (index: Nat := 0) (hop : opPtr.InBounds ctx)
     (hidx : index = opPtr.getNumResults ctx) : IRContext :=
-  match numResults with
-  | 0 => ctx
-  | Nat.succ n =>
-    let result: OpResult := { type := (), firstUse := none, index := index, owner := opPtr }
+  if h: index >= resultTypes.size then
+    ctx
+  else
+    let result: OpResult := { type := resultTypes[index], firstUse := none, index := index, owner := opPtr }
     let ctx := opPtr.pushResult ctx result
     have : opPtr.InBounds ctx := by grind
     have : result.FieldsInBounds ctx := by
       -- TODO(later): write the right lemma somewhere.
       constructor <;> grind [OperationPtr.pushResult, OperationPtr.setResults, OperationPtr.set, OperationPtr.get]
-    Rewriter.initOpResults ctx opPtr n (index + 1) (by grind) (by grind)
+    Rewriter.initOpResults ctx opPtr resultTypes (index + 1) (by grind) (by grind)
+  termination_by resultTypes.size - index
+  decreasing_by lia
 
 @[grind .]
 theorem Rewriter.initOpResults_fieldsInBounds (hx : ctx.FieldsInBounds) :
-    (initOpResults ctx opPtr numResults index h₁ h₂).FieldsInBounds := by
-  induction numResults generalizing ctx index
-  · grind [initOpResults]
-  case succ numResults ih =>
-    simp [initOpResults]
+    (initOpResults ctx opPtr resultTypes index h₁ h₂).FieldsInBounds := by
+  induction h: (resultTypes.size - index) generalizing index ctx
+  case zero =>
+    unfold initOpResults
+    grind
+  case succ resultTypes ih =>
+    unfold initOpResults
+    split; grind
     apply ih
-    apply OperationPtr.pushResult_fieldsInBounds
-    · constructor <;> grind [OperationPtr.pushResult, OperationPtr.setResults, OperationPtr.set, OperationPtr.get]
+    · apply OperationPtr.pushResult_fieldsInBounds
+      · constructor <;> grind [OperationPtr.pushResult, OperationPtr.setResults, OperationPtr.set, OperationPtr.get]
+      · grind
     · grind
 
 @[grind .]
 theorem Rewriter.initOpResults_inBounds_mono (ptr : GenericPtr) :
-    ptr.InBounds ctx → ptr.InBounds (initOpResults ctx opPtr numResults index h₁ h₂) := by
-  induction numResults generalizing ctx index <;> grind [initOpResults]
+    ptr.InBounds ctx → ptr.InBounds (initOpResults ctx opPtr resultTypes index h₁ h₂) := by
+  induction h: (resultTypes.size - index) generalizing index ctx <;> unfold initOpResults <;> grind
 
 @[irreducible]
 protected def Rewriter.pushOperand (ctx : IRContext) (opPtr : OperationPtr) (valuePtr : ValuePtr)
@@ -469,7 +474,7 @@ theorem Rewriter.createEmptyOp_fieldsInBounds (h : createEmptyOp ctx opType = so
 
 @[irreducible]
 def Rewriter.createOp (ctx: IRContext) (opType: Nat)
-    (numResults: Nat) (operands: Array ValuePtr) (regions: Array RegionPtr) (properties: UInt64)
+    (resultTypes: Array MlirType) (operands: Array ValuePtr) (regions: Array RegionPtr) (properties: UInt64)
     (insertionPoint: Option InsertPoint)
     (hoper : ∀ oper, oper ∈ operands → oper.InBounds ctx)
     (hregions : ∀ reg, reg ∈ regions → reg.InBounds ctx)
@@ -480,7 +485,7 @@ def Rewriter.createOp (ctx: IRContext) (opType: Nat)
   have : (newOpPtr.get ctx (by grind)).results = #[] := by
     grind [createEmptyOp, OperationPtr.allocEmpty, Operation.empty]
   have newOpPtrZeroRes: 0 = newOpPtr.getNumResults ctx (by grind) := by grind [OperationPtr.getNumResults]
-  let ctx := Rewriter.initOpResults ctx  newOpPtr numResults 0 hib newOpPtrZeroRes
+  let ctx := Rewriter.initOpResults ctx newOpPtr resultTypes 0 hib newOpPtrZeroRes
   let ctx := newOpPtr.setProperties ctx properties (by grind)
   have newOpPtrInBounds : newOpPtr.InBounds ctx := by grind
   let ctx := Rewriter.initOpRegions ctx newOpPtr regions
